theories/L/Complexity/Cook/SharedSAT.v
@@ -1,5 +1,5 @@
 From Undecidability.L Require Import L.
-From Undecidability.L.Datatypes Require Import LLists. 
+From Undecidability.L.Datatypes Require Import LLists LLNat. 
 Require Import Lia. 
 
 Notation var := (nat) (only parsing). 
@@ -11,3 +11,17 @@ Lemma evalVar_in_iff a v : evalVar a v = true <-> v el a.
 Proof. 
   unfold evalVar. rewrite list_in_decb_iff; [easy | symmetry; apply Nat.eqb_eq].
 Qed.
+
+Lemma evalVar_monotonic a a' v : a <<= a' -> evalVar a v = true -> evalVar a' v = true.
+Proof. 
+  intros H1 H2. rewrite evalVar_in_iff in *. firstorder.
+Qed. 
+
+Lemma evalVar_assgn_equiv a a' v : a === a' -> evalVar a v = evalVar a' v. 
+Proof. 
+  intros H. enough (evalVar a v = true <-> evalVar a' v = true).
+  { destruct evalVar, evalVar; firstorder. }
+  split; apply evalVar_monotonic; apply H. 
+Qed.
+
+
